properly add Rustan

Stuff/Rustan.lean
@@ -4,7 +4,7 @@ inductive E
 | lit : Bool → E
 | var : Nat → E
 | ite : E → E → E → E
-deriving BEq
+deriving DecidableEq
 
 def E.hasNestedIf : E → Bool
 | lit _ => false
@@ -47,11 +47,6 @@ def E.eval (f : Nat → Bool) : E → Bool
 | ite i t e => bif i.eval f then t.eval f else e.eval f
 
 open E
-
-def E.occs : E → List ℕ
-  | lit _ => []
-  | var v => List.ofFn (fun i : Fin (v+1) => if i = Fin.last _ then 1 else 0)
-  | ite i t e => List.zipWith (· + ·) (List.zipWith (· + ·) i.occs t.occs) e.occs
 
 def E.elimVar (v : ℕ) : E → (E × E)
   | lit b => (lit b, lit b)
@@ -134,8 +129,106 @@ theorem E.disjointLE_of_le {v w : ℕ} (h : v ≤ w) :
             E.disjointLE_of_le h ht,
             E.disjointLE_of_le h he⟩
 
+theorem E.disjointLE_elimVar_fst {v : ℕ} :
+    ∀ (e : E), (∀ w < v, disjointLE w e) ↔ disjointLE v (e.elimVar v).1
+  | lit _ => by simp [elimVar, disjointLE]
+  | var w => by
+    simp [elimVar, disjointLE]
+    split_ifs
+    · simp [disjointLE]
+    · simp [disjointLE]
+  | ite i t e => by
+    simp only [disjointLE, Bool.and_eq_true, forall_and,
+      vars_elimVar_fst, vars_elimVar_snd,
+      i.disjointLE_elimVar_fst,
+      t.disjointLE_elimVar_fst,
+      e.disjointLE_elimVar_fst,
+      ← and_assoc, and_congr_left_iff]
+    intros _ _ _
+    simp [List.disjoint_iff, List.mem_filter, decide_eq_true]
+    refine and_congr ?_ ?_
+    . refine ⟨fun h x hxi hxv hvx hxt =>
+        (h x (lt_of_le_of_ne hxv (Ne.symm hvx)) x hxi (le_refl x) hxt).elim,
+        fun h x hxv y hyi hyx hyt => ne_of_lt (lt_of_le_of_lt hyx hxv)
+          (Eq.symm (h y hyi (le_trans hyx (le_of_lt hxv))
+          (Ne.symm (ne_of_lt (lt_of_le_of_lt hyx hxv))) hyt))⟩
+    · refine ⟨fun h x hxi hxv hvx hxt =>
+        (h x (lt_of_le_of_ne hxv (Ne.symm hvx)) x hxi (le_refl x) hxt).elim,
+        fun h x hxv y hyi hyx hyt => ne_of_lt (lt_of_le_of_lt hyx hxv)
+          (Eq.symm (h y hyi (le_trans hyx (le_of_lt hxv))
+          (Ne.symm (ne_of_lt (lt_of_le_of_lt hyx hxv))) hyt))⟩
+
+theorem E.disjointLE_elimVar_snd {v : ℕ} :
+    ∀ (e : E), (∀ w < v, disjointLE w e) ↔ disjointLE v (e.elimVar v).2
+  | lit _ => by simp [elimVar, disjointLE]
+  | var w => by
+    simp [elimVar, disjointLE]
+    split_ifs
+    · simp [disjointLE]
+    · simp [disjointLE]
+  | ite i t e => by
+    simp only [disjointLE, Bool.and_eq_true, forall_and,
+      vars_elimVar_snd, vars_elimVar_snd,
+      i.disjointLE_elimVar_snd,
+      t.disjointLE_elimVar_snd,
+      e.disjointLE_elimVar_snd,
+      ← and_assoc, and_congr_left_iff]
+    intros _ _ _
+    simp [List.disjoint_iff, List.mem_filter, decide_eq_true]
+    refine and_congr ?_ ?_
+    . refine ⟨fun h x hxi hxv hvx hxt =>
+        (h x (lt_of_le_of_ne hxv (Ne.symm hvx)) x hxi (le_refl x) hxt).elim,
+        fun h x hxv y hyi hyx hyt => ne_of_lt (lt_of_le_of_lt hyx hxv)
+          (Eq.symm (h y hyi (le_trans hyx (le_of_lt hxv))
+          (Ne.symm (ne_of_lt (lt_of_le_of_lt hyx hxv))) hyt))⟩
+    · refine ⟨fun h x hxi hxv hvx hxt =>
+        (h x (lt_of_le_of_ne hxv (Ne.symm hvx)) x hxi (le_refl x) hxt).elim,
+        fun h x hxv y hyi hyx hyt => ne_of_lt (lt_of_le_of_lt hyx hxv)
+          (Eq.symm (h y hyi (le_trans hyx (le_of_lt hxv))
+          (Ne.symm (ne_of_lt (lt_of_le_of_lt hyx hxv))) hyt))⟩
+
+@[simp]
+theorem E.hasNestedIf_elimVar_fst (v : ℕ) :(e : E) →
+    hasNestedIf (elimVar v e).1 = hasNestedIf e
+  | lit _ => by simp [elimVar, hasNestedIf]
+  | var _ => by
+    simp [elimVar, hasNestedIf]
+    split_ifs <;> simp [hasNestedIf]
+  | .ite (.ite _ _ _) _ _ => by
+    simp [hasNestedIf, elimVar]
+  | .ite (lit _) t e => by
+    simp [hasNestedIf, elimVar, t.hasNestedIf_elimVar_fst,
+      e.hasNestedIf_elimVar_fst]
+  | .ite (var _) t e => by
+    simp [hasNestedIf, elimVar, t.hasNestedIf_elimVar_fst,
+      e.hasNestedIf_elimVar_fst]
+    split_ifs <;>
+    simp [hasNestedIf, elimVar, t.hasNestedIf_elimVar_fst,
+      e.hasNestedIf_elimVar_fst]
+
+@[simp]
+theorem E.hasNestedIf_elimVar_snd (v : ℕ) :(e : E) →
+    hasNestedIf (elimVar v e).2 = hasNestedIf e
+  | lit _ => by simp [elimVar, hasNestedIf]
+  | var _ => by
+    simp [elimVar, hasNestedIf]
+    split_ifs <;> simp [hasNestedIf]
+  | .ite (.ite _ _ _) _ _ => by
+    simp [hasNestedIf, elimVar]
+  | .ite (lit _) t e => by
+    simp [hasNestedIf, elimVar, t.hasNestedIf_elimVar_snd,
+      e.hasNestedIf_elimVar_snd]
+  | .ite (var _) t e => by
+    simp [hasNestedIf, elimVar, t.hasNestedIf_elimVar_snd,
+      e.hasNestedIf_elimVar_snd]
+    split_ifs <;>
+    simp [hasNestedIf, elimVar, t.hasNestedIf_elimVar_snd,
+      e.hasNestedIf_elimVar_snd]
+
 def E.dedupLE (v : ℕ) : (e : E) → (h : ∀ w < v, e.disjointLE w) →
-    { e' : E // e'.eval = e.eval ∧ e'.disjointLE v}
+    { e' : E // (∀ f, e'.eval f = e.eval f) ∧ e'.disjointLE v ∧
+        (∀ w, v < w → w ∈ e'.vars → w ∈ e.vars)
+        ∧ (!e.hasNestedIf → !e'.hasNestedIf) }
   | lit b, _ => ⟨lit b, by simp [disjointLE, eval]⟩
   | var i, _ => ⟨var i, by simp [disjointLE, eval]⟩
   | ite i t e, h =>
@@ -143,7 +236,7 @@ def E.dedupLE (v : ℕ) : (e : E) → (h : ∀ w < v, e.disjointLE w) →
     let t' := t.elimVar v
     let e' := e.elimVar v
     ⟨ite (var v) (ite i'.1 t'.1 e'.1) (ite i'.2 t'.2 e'.2), by
-      ext f
+      intro f
       simp [eval, eval_elimVar_fst, eval_elimVar_snd]
       by_cases hfv : f v = true
       · simp [hfv]
@@ -152,13 +245,264 @@ def E.dedupLE (v : ℕ) : (e : E) → (h : ∀ w < v, e.disjointLE w) →
       · simp [eq_false_of_ne_true hfv]
         congr <;>
         ext <;> split_ifs <;> simp_all, by
-    simp [disjointLE, E.vars_elimVar_snd, E.disjoint, E.vars,
-      E.vars_elimVar_fst, List.disjoint_iff, List.mem_filter] at h ⊢
+      simp
+        [disjointLE, E.vars_elimVar_snd, E.disjoint, E.vars, and_assoc,
+          E.vars_elimVar_fst, List.disjoint_iff, List.mem_filter] at h ⊢
+      have h₁ : ∀ (x : ℕ), x ∈ vars i → x ≤ v → ¬v = x → x ∈ vars t → v = x := by
+        intro x hxi hxv hvx hxt
+        exact ((h x (lt_of_le_of_ne hxv (Ne.symm hvx))).1 x hxi (le_refl x) hxt).elim
+      have h₂ : ∀ (x : ℕ), x ∈ vars i → x ≤ v → ¬v = x → x ∈ vars e → v = x := by
+        intro x hxi hxv hvx hxe
+        exact ((h x (lt_of_le_of_ne hxv (Ne.symm hvx))).2.1 x hxi (le_refl x) hxe).elim
+      simp only [← disjointLE_elimVar_fst, ← disjointLE_elimVar_snd]
+      simp only [forall_and] at h
+      refine ⟨h₁, h₂, ?_, ?_, ?_, h₁, h₂, ?_⟩ <;> tauto, by
+      simp [vars, vars_elimVar_fst, vars_elimVar_snd,
+        List.mem_filter, or_imp]
+      intro w hvw
+      simp [ne_of_gt hvw, ne_of_lt hvw]
+      tauto, by
+      simp [hasNestedIf]
+      cases i
+      · simp (config := {contextual := true}) [hasNestedIf]
+      · simp [hasNestedIf, elimVar]
+        split_ifs <;> simp (config := {contextual := true}) [hasNestedIf]
+      · simp [hasNestedIf, elimVar]⟩
 
+theorem E.lt_disjointLE_iff_disjointLE_of_not_mem_vars {v : ℕ} : ∀ {e : E},
+    (he : v ∉ e.vars) → (∀ w < v, e.disjointLE w) ↔ e.disjointLE v
+  | lit _ => by simp [disjointLE]
+  | var w => by simp [disjointLE]
+  | ite i t e => by
+    simp only [disjointLE, vars, List.mem_append, not_or,
+      and_imp, Bool.and_eq_true, List.disjoint_iff, List.mem_filter,
+      decide_eq_true_iff]
+    intro hvi hvt hve
+    simp only [forall_and, ← and_assoc,
+       ← i.lt_disjointLE_iff_disjointLE_of_not_mem_vars hvi,
+       ← t.lt_disjointLE_iff_disjointLE_of_not_mem_vars hvt,
+       ← e.lt_disjointLE_iff_disjointLE_of_not_mem_vars hve]
+    simp only [and_congr_left_iff]
+    intros h₁ h₂ h₃
+    refine and_congr ?_ ?_
+    . exact ⟨fun h x hxi hxv hxt =>
+      h x (lt_of_le_of_ne hxv (by rintro rfl; simp_all))
+        x hxi (le_refl _) hxt, fun h x hxv y hyi hyx hyt =>
+        h y hyi (le_trans hyx (le_of_lt hxv)) hyt⟩
+    . exact ⟨fun h x hxi hxv hxt =>
+      h x (lt_of_le_of_ne hxv (by rintro rfl; simp_all))
+        x hxi (le_refl _) hxt, fun h x hxv y hyi hyx hyt =>
+        h y hyi (le_trans hyx (le_of_lt hxv)) hyt⟩
 
-    ⟩
+theorem E.lt_disjointLE_iff_disjointLE_of_not_mem_vars' : ∀ {v : ℕ} {e : E},
+    (he : v ∉ e.vars) → (∀ w < v, w ∈ e.vars → e.disjointLE w) ↔ e.disjointLE v
+  | v, e, he => by
+    conv_rhs => rw [← E.lt_disjointLE_iff_disjointLE_of_not_mem_vars he]
+    refine ⟨?_, ?_⟩
+    · rintro h w hwv
+      by_cases hw : w ∈ e.vars
+      · exact h w hwv hw
+      · rw [← E.lt_disjointLE_iff_disjointLE_of_not_mem_vars' hw]
+        intro x hxw hxe
+        exact h x (lt_of_le_of_lt (le_of_lt hxw) hwv) hxe
+    · intro h w hwv _
+      exact h w hwv
 
+theorem E.disjoint_iff_disjointLE : ∀ {e : E}, e.disjoint ↔ ∀ v, e.disjointLE v
+  | lit _ => by simp [disjoint, disjointLE]
+  | var _ => by simp [disjoint, disjointLE]
+  | E.ite i t e => by
+    simp only [disjoint, disjointLE, i.disjoint_iff_disjointLE,
+      t.disjoint_iff_disjointLE, e.disjoint_iff_disjointLE,
+      List.disjoint_iff, decide_eq_true_iff, Bool.and_eq_true,
+      E.vars, List.mem_append, or_assoc, List.mem_filter,
+      and_imp, and_assoc]
+    refine ⟨?_, ?_⟩
+    · intro h v
+      tauto
+    · intro h
+      simp only [← forall_and, and_assoc]
+      intro v
+      have := h v
+      have h₁ := this.1 v
+      have h₂ := this.2.1 v
+      simp at h₁ h₂
+      tauto
+
+def E.dedupAllLE : (v : ℕ) → (e : E) →
+    { e' : E // (∀ f, e'.eval f = e.eval f) ∧ e'.disjointLE v ∧
+      (∀ w, v < w → w ∈ e'.vars → w ∈ e.vars) ∧
+      (!e.hasNestedIf → !e'.hasNestedIf) }
+  | 0, e => e.dedupLE 0 (by simp)
+  | v+1, e =>
+    let e' := E.dedupAllLE v e
+    let e'' := @E.dedupLE (v+1) e' (fun w hw =>
+      E.disjointLE_of_le (Nat.le_of_lt_succ hw) e'.2.2.1)
+    ⟨e''.1, fun _ => by rw [e''.2.1, e'.2.1], e''.2.2.1,
+      fun w hvw hwe => by
+      have := e''.2.2.2.1 w hvw hwe
+      exact e'.2.2.2.1 w (Nat.lt_of_succ_lt hvw) this, by
+      intro h
+      apply e''.2.2.2.2
+      exact e'.2.2.2.2 h⟩
+
+def List.leastGE : (l : List ℕ) → {n : ℕ // ∀ m ∈ l, m ≤ n}
+  | [] => ⟨0, by simp⟩
+  | a::l =>
+    let m := List.leastGE l
+    if ham : a ≤ m then ⟨m.1, by
+      intro k
+      rw [List.mem_cons]
+      rintro (rfl | hkl)
+      · exact ham
+      · exact m.2 _ hkl⟩
+    else ⟨a, by
+      intro k
+      rw [List.mem_cons]
+      rintro (rfl | hkl)
+      · exact le_refl _
+      · exact le_trans (m.2 _ hkl) (le_of_not_ge ham)⟩
+
+def E.dedup (e : E) : { e' : E // (∀ f, e'.eval f = e.eval f) ∧ e'.disjoint ∧
+      (!e.hasNestedIf → !e'.hasNestedIf) } :=
+  let v := List.leastGE e.vars
+  let e' := E.dedupAllLE v e
+  ⟨e'.1, e'.2.1, by
+    rw [E.disjoint_iff_disjointLE]
+    intro w
+    by_cases hw : w ≤ v.1
+    · exact disjointLE_of_le hw e'.2.2.1
+    · have hw : w ∉ e'.1.vars := by
+        intro hwe
+        have := e'.2.2.2.1 w (lt_of_not_ge hw) hwe
+        exact hw (v.2 _ this)
+      rw [← E.lt_disjointLE_iff_disjointLE_of_not_mem_vars' hw]
+      intro x _ hxe'
+      refine disjointLE_of_le ?_ e'.2.2.1
+      refine le_of_not_lt ?_
+      intro hvx
+      have := e'.2.2.2.1 _ hvx hxe'
+      have := v.2 _ this
+      exact not_le_of_gt hvx this,  e'.2.2.2.2⟩
+
+@[simp]
+def E.denestSize : E → ℕ
+  | lit _ => 0
+  | var _ => 0
+  | .ite i t e =>
+    2 * E.denestSize i +
+      max (E.denestSize t) (E.denestSize e) + 1
+
+def E.denest : (e : E) → { e' : E // (∀ f, e'.eval f = e.eval f) ∧ !e'.hasNestedIf }
+  | lit b => ⟨lit b, by simp [eval, hasNestedIf]⟩
+  | var i => ⟨var i, by simp [eval, hasNestedIf]⟩
+  | .ite (.ite a b c) d e =>
+      have : 2 * denestSize a +
+          max (2 * denestSize b + max (denestSize d) (denestSize e) + 1)
+          (2 * denestSize c + max (denestSize d) (denestSize e) + 1) <
+          2 * (2 * denestSize a + max (denestSize b) (denestSize c) + 1) +
+          max (denestSize d) (denestSize e) := by
+        simp only [denestSize, add_assoc, add_lt_add_iff_left]
+        simp only [← add_assoc, max_add_add_right]
+        simp only [← two_mul, max_mul_mul_left]
+        linarith
+      have ⟨t', ht'⟩ := E.denest (.ite a (.ite b d e) (.ite c d e))
+      ⟨t', by
+        simp [eval, ht'.1, ht'.2, hasNestedIf]
+        intro f
+        cases eval f a <;> simp⟩
+  | .ite (lit true) t e =>
+    have : denestSize t < 2 + max (denestSize t) (denestSize e) + 1 :=
+      calc denestSize t < max (denestSize t) (denestSize e) + 3 :=
+        Nat.lt_succ_of_le (le_add_right (le_max_left _ _))
+      _ = _ := by ring
+    ⟨E.denest t, by simp [eval, hasNestedIf, (E.denest t).2]⟩
+  | .ite (lit false) t e =>
+    have : denestSize e < 2 + max (denestSize t) (denestSize e) + 1 :=
+      calc denestSize e < max (denestSize t) (denestSize e) + 3 :=
+        Nat.lt_succ_of_le (le_add_right (le_max_right _ _))
+      _ = _ := by ring
+    ⟨E.denest e, by simp [eval, hasNestedIf, (E.denest e).2]⟩
+  | .ite (var v) t e =>
+    have : denestSize t < 2 + max (denestSize t) (denestSize e) + 1 :=
+      calc denestSize t < max (denestSize t) (denestSize e) + 3 :=
+        Nat.lt_succ_of_le (le_add_right (le_max_left _ _))
+      _ = _ := by ring
+    have : denestSize e < 2 + max (denestSize t) (denestSize e) + 1 :=
+      calc denestSize e < max (denestSize t) (denestSize e) + 3 :=
+        Nat.lt_succ_of_le (le_add_right (le_max_right _ _))
+      _ = _ := by ring
+    have ⟨t', ht'⟩ := E.denest t
+    have ⟨e', he'⟩ := E.denest e
+    ⟨.ite (var v) t' e', by
+      simp [eval, ht'.1, ht'.2, he'.1, he'.2, hasNestedIf]⟩
+  termination_by E.denest e => e.denestSize
+
+def E.deConstRed : (e : E) → { e' : E //
+    e.disjoint → !e.hasNestedIf →
+    (∀ f, e'.eval f = e.eval f) ∧
+    !e'.hasConstantIf ∧
+    (!e'.hasNestedIf) ∧
+    ( e'.disjoint) ∧
+    (!e'.hasRedundantIf) ∧
+    e'.vars ⊆ e.vars }
+  | lit b => ⟨lit b, by
+    simp (config := {contextual := true}) [eval, hasConstantIf, hasRedundantIf]⟩
+  | var i => ⟨var i, by
+    simp (config := {contextual := true}) [eval, hasConstantIf, hasRedundantIf]⟩
+  | .ite (lit true) t e =>
+    have ⟨t', ht'⟩ := E.deConstRed t
+    ⟨t', by
+      simp [Function.funext_iff, disjoint, vars, eval, hasRedundantIf,
+        List.disjoint, hasNestedIf, List.subset_def] at *
+      tauto
+      ⟩
+  | .ite (lit false) t e =>
+    have ⟨e', he'⟩ := E.deConstRed e
+    ⟨e', by
+      simp [Function.funext_iff, disjoint, vars, eval, hasRedundantIf,
+        List.disjoint, hasNestedIf, List.subset_def] at *
+      tauto
+      ⟩
+  | .ite (var v) t e =>
+    have ⟨t', ht'⟩ := E.deConstRed t
+    have ⟨e', he'⟩ := E.deConstRed e
+    if hte' : t' = e'
+    then ⟨t', by
+      subst hte'
+      simp [Function.funext_iff, disjoint, vars, eval, hasRedundantIf,
+        List.disjoint, hasNestedIf, List.subset_def] at *
+      aesop
+      ⟩
+    else
+    ⟨.ite (var v) t' e', by
+      simp [Function.funext_iff, disjoint, vars, eval, List.subset_def,
+        List.disjoint, hasNestedIf, hasConstantIf, hasRedundantIf] at *
+      intro _ _ _ _ _ _
+      refine ⟨?_, ?_⟩
+      · intro f
+        cases hf : f v <;> simp_all
+      · aesop⟩
+  | .ite (.ite a b c) t e =>
+    ⟨.ite (.ite a b c) t e, by
+      simp [Function.funext_iff, disjoint, vars, eval, List.subset_def,
+        List.disjoint, hasNestedIf, hasConstantIf] at *⟩
+
+def E.normalize (e : E) : { e' : E // e'.normalized ∧ ∀ f, e'.eval f = e.eval f } :=
+  have ⟨e₁, he₁⟩ := e.denest
+  have ⟨e₂, he₂⟩ := e₁.dedup
+  have ⟨e₃, he₃⟩ := e₂.deConstRed
+  ⟨e₃, by
+    refine ⟨?_, ?_⟩
+    · simp only [normalized, Bool.and_eq_true]
+      aesop
+    · intro f
+      simp_all⟩
 
 def IfNormalization : Type := { Z : E → E // ∀ e, (Z e).normalized ∧ ∀ f, (Z e).eval f = e.eval f }
 
-example : IfNormalization := sorry
+example : IfNormalization :=
+  ⟨fun e => e.normalize, by
+    intro e
+    exact ⟨e.normalize.2.1, by
+      simpa [Function.funext_iff] using e.normalize.2.2⟩⟩
